coq/theories/Syntax.v
@@ -28,22 +28,26 @@ Inductive exp: Set :=
 
 Inductive cmd: Set :=
 | Assign (x: name) (e: exp)
-| Block (cs: list cmd)
+| Nop
+| Seq (c1 c2: cmd)
 | If (e: exp) (c1 c2: cmd)
 | Extr (x: name)
 | Emit (x: name)
-| Apply (t: name)
-| Call (a: name) (args: list exp).
+| Apply (t: name).
 
 Inductive typ: Set :=
 | Bit (n: nat)
 | Bool
 | Prod (ts: list typ).
 
+Inductive action :=
+| ActAssign (x: name) (e: exp)
+| ActSeq (a1 a2: action)
+| ActNop.
+
 Inductive defn: Set :=
 | VarDecl (t: typ) (x: name) (e: exp)
-| Action (a: name) (params: list (name * typ)) (c: cmd)
-| Table (t: name) (keys: exp) (actions: list name).
+| Table (t: name) (keys: exp) (acts: list action).
 
 Definition prog: Set :=
   list defn * cmd.
@@ -53,23 +57,18 @@ Inductive val: Set :=
 | VBool (b: bool)
 | VTuple (vs: list val).
 
-Record action :=
-  { params: list (name * typ);
-    body: cmd }.
-
 Record rule :=
   { rule_match: exp;
-    rule_action: name;
-    rule_args: list val }.
+    rule_action: nat }.
 
 Record table :=
-  { table_key: exp;
-    table_acts: list name; }.
+  { table_key: exp; table_acts: list action }.
+
+Record def_state :=
+  { type_env: Env.t name typ;
+    tables: Env.t name table;
+    rules: Env.t name (list rule) }.
 
 Record state :=
   { store: Env.t name val;
-    type_env: Env.t name typ;
-    pkt: list bool;
-    acts: Env.t name action;
-    tables: Env.t name table;
-    rules: Env.t name (list rule) }.
+    pkt: list bool }.
